coqimp/contextswitch/lib/derived_rule.v
@@ -1,0 +1,82 @@
+Require Import Coqlib.             
+Require Import Maps.       
+Require Import LibTactics.  
+        
+Require Import Integers.  
+Open Scope Z_scope.     
+Import ListNotations. 
+  
+Set Asymmetric Patterns.  
+       
+Require Import state.    
+Require Import language. 
+ 
+Set Implicit Arguments.    
+Unset Strict Implicit. 
+              
+Require Import logic.
+   
+Require Import lemmas.
+Require Import lemmas_ins.
+
+Require Import Coq.Logic.FunctionalExtensionality.
+
+Require Import sep_lemma.
+Require Import reg_lemma.
+
+Open Scope nat.
+Open Scope code_scope.
+Open Scope mem_scope.
+  
+Print wf_seq.
+
+Theorem forward_rule :
+  forall p q q' Spec I,
+    q ==> q' ->
+    Spec |- {{ p }} I {{ q }} ->
+    Spec |- {{ p }} I {{ q' }}.
+Proof.
+  intros.
+  eapply Seq_conseq_rule; eauto.
+Qed.
+
+Theorem backward_rule :
+  forall p p' q Spec I,
+    p' ==> p ->
+    Spec |- {{ p }} I {{ q }} ->
+    Spec |- {{ p' }} I {{ q }}.
+Proof.
+  intros.
+  eapply Seq_conseq_rule; eauto.
+Qed.
+  
+Theorem ex_intro_rule' :
+  forall I {tp : Type} (p q : tp -> asrt) (Spec : funspec),
+    (forall x' : tp, Spec |- {{ p x' }} I {{ q x' }}) ->
+    Spec |- {{ EX x : tp, p x }} I {{ EX x : tp, q x }}.
+Proof.
+  intros.
+  eapply Ex_intro_rule; eauto.
+  intros. 
+  eapply forward_rule; [idtac | eauto].
+  intros.
+  simpl.
+  eauto.
+Qed.
+
+Ltac hoare_ex_intro :=
+  match goal with
+  | |- _ |- {{ EX _, _ }} _ {{ EX _, _ }} =>
+    eapply ex_intro_rule'; try intros;
+    hoare_ex_intro
+  | _ => idtac
+  end.
+
+Ltac hoare_lift_pre n :=
+  let H' := fresh in
+  match goal with
+  | |- _ |- {{ _ }} _ {{ _ }} =>
+    eapply backward_rule;
+    [ introv H'; simpl_sep_liftn_in H' n; eapply H' | idtac]
+  | _ => idtac
+  end.
